# 2024.9.25 刷题记录

## P46 选择题

| 1    | 2    | 3    | 4    |
| ---- | ---- | ---- | ---- |
| C    | D    | D    | A    |



## P47 填空题

### 1. 

$$
\frac{dy}{dx}=2xy,f(0)=2\\
\frac{dy}y=2xdx,\\
\ln y=x^2+C_1,\\
y=Ce^{x^2},C=2\\
f(x)=2e^{x^2}
$$



### 2.

$$
dy=\frac{xy}{1+x^2}dx\\
\frac{dy}{y}=\frac{x}{1+x^2}dx\\
\ln y=\int\frac{xdx}{1+x^2}=\frac12\ln(1+x^2)+C'\\
y=C\sqrt{1+x^2},y(0)=C=2\\
y(x)=2\sqrt{1+x^2}
$$

### 3.

$$
(1+y^2)dx-2xydy=0\\
\frac{y}{1+y^2}dy=\frac{dx}{2x}\\
\frac12\ln(1+y^2)=\frac12\ln x+C\\
y(1)=0,\frac12\ln(1+0)=\frac12\ln1+C,C=0\\
\ln(1+y^2)=\ln x\\
x=1+y^2
$$

### 4. 

$$
y'-\frac2x y=1\\
y=e^{\int\frac2xdx}(C+\int e^{-\int\cfrac2xdx}dx)=\\
e^{2\ln x}(C+e^{-2\ln x})\\
y=Cx^2+1
$$

### 5.

$$
p=\frac12,q=\frac12
$$

### 6.

$$
-\int_0^x f(x-t)dt=\int_0^x(x-t)d(x-t)=\int_x^0f(u)du=-\int_0^xf(u)du\\
f'(x)-f(x)=e^x\\
f(x)=e^x(C+x)\\
f(0)=1,C=1,f(x)=xe^x+e^x
$$

### 7. 

特征方程：$r^2-r=0$，齐次通解：
$$
C_1e^x+C_2
$$
$y''-y'=(2x+1)e^x$ 的 $\lambda=1,P_m=2x+1$，特解为
$$
R(x)=xP_m=2x^2+x,e^x(2x^2+x)
$$
$y''-y'=4x-1$ 的 $\lambda=0,P_m=4x-1$，特解为：
$$
R(x)=xP_m=4x^2-x
$$
通解：
$$
C_1e^x+C_2+e^x(2x^2+x)+4x^2-x
$$


### 8. 

$$
12e^{2x}+6pe^{2x}+2q+3qe^{2x}=0\\
q=0\\
p=-2\\
y''-2y'=0
$$

### 9.

$$
r^2+qr+p=-\\
q^2=4p\\
-\frac q2=1\\
q=-2,p=1\\
y''+y'-2y=0
$$

### 10.

$$
y'-y=y^2,P(x)=-1,Q(x)=1,n=2,\\
z=y^{1-2}=y^{-1}\\
z'+z=-1\\
z=e^{-x}(C-e^x)\\
y=e^x\frac1{C-e^x},C=-1\\
y'=-\frac{e^x}{1+e^x}\\
y=-\ln(1+e^x)+C,C=0\\
y=-\ln(1+e^x)
$$

### 11.

$$
x=e^t,\frac{dx}{dt}=e^t,dx=e^tdt\\
x^2\frac{d^2y}{dx^2}+x\frac{dy}{dx}-y=0\\
x^2\frac{d^2y}{e^{2t}dt^2}+x\frac{dy}{e^tdt}-4y=
\frac{d^2y}{dt^2}+\frac{dy}{dt}-4y=0\\
特征方程:r^2+r-4=0\\
r=\frac{-1\pm\sqrt{17}}{2}\\
y=C_1\exp{\frac{-1+\sqrt{17}}{2}t}+C_2\exp{\frac{-1-\sqrt{17}}{2}t}\\
t=\ln x\\
y=C_1x^{\cfrac{-1+\sqrt{17}}{2}}+C_2x^{\cfrac{-1-\sqrt{17}}{2}}
$$

### 12.

$$
\frac1{y^2}\frac{dy}{dx}+\frac2x\frac1{y}=x\\
z=-\frac 1y\\
z'-\frac2xz=x\\
z=e^{\int\frac2xdx}(C+\int e^{-\int\frac2xdx}xdx)=\\
e^{2\ln x}(C+\int e^{-2\ln x}xdx)=\\
x^2(C+\int x^{-1}dx)=Cx^2+x^2\ln x\\
$$

